James C - cleaned 12, 15, 16

isabelle/Chapter12_1_Language.thy
@@ -71,64 +71,34 @@ primrec mult_insert :: "nat => expr => expr"
 where "mult_insert 0 e = e"
     | "mult_insert (Nat.Suc n) e = insert first (mult_insert n e)"
 
-primrec remove :: "var => expr => expr"
-    and remove_rules :: "var => rule list => rule list"
-    and remove_rule :: "var => rule => rule"
-where "remove n (Var v) = Var (subr n v)"
-    | "remove n Zero = Zero"
-    | "remove n (Suc e) = Suc (remove n e)"
-    | "remove n (Rec et e0 es) = Rec (remove n et) (remove n e0) (remove (next (next n)) es)"
-    | "remove n (Lam t e) = Lam t (remove (next n) e)"
-    | "remove n (Appl e1 e2) = Appl (remove n e1) (remove n e2)"
-    | "remove n Triv = Triv"
-    | "remove n (Pair e1 e2) = Pair (remove n e1) (remove n e2)"
-    | "remove n (ProjL e) = ProjL (remove n e)"
-    | "remove n (ProjR e) = ProjR (remove n e)"
-    | "remove n (Abort t e) = Abort t (remove n e)"
-    | "remove n (Case et el er) = Case (remove n et) (remove (next n) el) (remove (next n) er)"
-    | "remove n (InL t1 t2 e) = InL t1 t2 (remove n e)"
-    | "remove n (InR t1 t2 e) = InR t1 t2 (remove n e)"
-    | "remove n (Match e rs) = Match (remove n e) (remove_rules n rs)"
-    | "remove_rules n [] = []"
-    | "remove_rules n (r # rs) = remove_rule n r # remove_rules n rs"
-    | "remove_rule n (Rule p e) = Rule p (remove (next_by (pat_var_count p) n) e)"
-
-primrec subst' :: "var => expr => expr => expr"
-    and subst_rules :: "var => expr => rule list => rule list"
-    and subst_rule :: "var => expr => rule => rule"
-where "subst' n e' (Var v) = (if v = n then e' else Var v)"
-    | "subst' n e' Zero = Zero"
-    | "subst' n e' (Suc e) = Suc (subst' n e' e)"
-    | "subst' n e' (Rec et e0 es) = 
-                      Rec (subst' n e' et) 
-                          (subst' n e' e0) 
-                          (subst' (next (next n)) (insert first (insert first e')) es)"
-    | "subst' n e' (Lam t e) = Lam t (subst' (next n) (insert first e') e)"
-    | "subst' n e' (Appl e1 e2) = Appl (subst' n e' e1) (subst' n e' e2)"
-    | "subst' n e' Triv = Triv"
-    | "subst' n e' (Pair e1 e2) = Pair (subst' n e' e1) (subst' n e' e2)"
-    | "subst' n e' (ProjL e) = ProjL (subst' n e' e)"
-    | "subst' n e' (ProjR e) = ProjR (subst' n e' e)"
-    | "subst' n e' (Abort t e) = Abort t (subst' n e' e)"
-    | "subst' n e' (Case et el er) = 
-                      Case (subst' n e' et) 
-                           (subst' (next n) (insert first e') el) 
-                           (subst' (next n) (insert first e') er)"
-    | "subst' n e' (InL t1 t2 e) = InL t1 t2 (subst' n e' e)"
-    | "subst' n e' (InR t1 t2 e) = InR t1 t2 (subst' n e' e)"
-    | "subst' n e' (Match e rs) = Match (subst' n e' e) (subst_rules n e' rs)"
-    | "subst_rules n e' [] = []"
-    | "subst_rules n e' (r # rs) = subst_rule n e' r # subst_rules n e' rs"
-    | "subst_rule n e' (Rule p e) = Rule p (subst' (next_by (pat_var_count p) n) 
-                                                   (mult_insert (pat_var_count p) e') e)"
-
-definition subst :: "expr => var => expr => expr"
-where "subst e' n e = remove first (subst' first (insert first e') e)"
-
-lemma [simp]: "remove n (insert n e) = e"
-  and [simp]: "remove_rules n (insert_rules n rs) = rs"
-  and [simp]: "remove_rule n (insert_rule n r) = r"
-by (induction e and rs and r arbitrary: n and n and n, simp_all)
+primrec subst :: "expr => var => expr => expr"
+    and subst_rules :: "expr => var => rule list => rule list"
+    and subst_rule :: "expr => var => rule => rule"
+where "subst e' n (Var v) = (if v = n then e' else Var (subr n v))"
+    | "subst e' n Zero = Zero"
+    | "subst e' n (Suc e) = Suc (subst e' n e)"
+    | "subst e' n (Rec et e0 es) = 
+                      Rec (subst e' n et) 
+                          (subst e' n e0) 
+                          (subst (insert first (insert first e')) (next (next n)) es)"
+    | "subst e' n (Lam t e) = Lam t (subst (insert first e') (next n) e)"
+    | "subst e' n (Appl e1 e2) = Appl (subst e' n e1) (subst e' n e2)"
+    | "subst e' n Triv = Triv"
+    | "subst e' n (Pair e1 e2) = Pair (subst e' n e1) (subst e' n e2)"
+    | "subst e' n (ProjL e) = ProjL (subst e' n e)"
+    | "subst e' n (ProjR e) = ProjR (subst e' n e)"
+    | "subst e' n (Abort t e) = Abort t (subst e' n e)"
+    | "subst e' n (Case et el er) = 
+                      Case (subst e' n et) 
+                           (subst (insert first e') (next n) el) 
+                           (subst (insert first e') (next n) er)"
+    | "subst e' n (InL t1 t2 e) = InL t1 t2 (subst e' n e)"
+    | "subst e' n (InR t1 t2 e) = InR t1 t2 (subst e' n e)"
+    | "subst e' n (Match e rs) = Match (subst e' n e) (subst_rules e' n rs)"
+    | "subst_rules e' n [] = []"
+    | "subst_rules e' n (r # rs) = subst_rule e' n r # subst_rules e' n rs"
+    | "subst_rule e' n (Rule p e) = Rule p (subst (mult_insert (pat_var_count p) e') 
+                                                  (next_by (pat_var_count p) n) e)"
 
 lemma [simp]: "canswap m n ==> insert m (insert n e) = insert (next n) (insert m e)"
   and [simp]: "canswap m n ==> 
